Intermediate commit

Test/Tests/Groups.lean
@@ -3,27 +3,56 @@ import Egg
 -- TODO: This set of test cases seems to demonstrate that `typeTags ≠ .none` is way too slow or
 --       doesn't work.
 
--- TODO: What happens when G is defined as a class?
+class Group (α) where
+  zero          : α
+  neg           : α → α
+  add           : α → α → α
+  add_assoc     : ∀ a b c, add (add a b) c = add a (add b c)
+  zero_add      : ∀ a, add zero a = a
+  add_zero      : ∀ a, add a zero = a
+  add_left_inv  : ∀ a, add (neg a) a = zero
+  add_right_inv : ∀ a, add a (neg a) = zero
 
-def G : Type := sorry
-def zero : G := sorry
-def neg : G → G := sorry
-def add : G → G → G := sorry
+open Group
 
-instance : Neg G where neg := neg
-instance : Add G where add := add
-instance : OfNat G 0 where ofNat := zero
+instance [Group α] : Neg α where neg := neg
+instance [Group α] : Add α where add := add
+instance [Group α] : OfNat α 0 where ofNat := zero
 
-variable {a b c : G}
+variable [g : Group G] {a b c : G}
 
-theorem add_assoc     : (a + b) + c = a + (b + c) := by sorry
-theorem zero_add      : 0 + a = a                 := by sorry
-theorem add_zero      : a + 0 = a                 := by sorry
-theorem add_left_inv  : -a + a = 0                := by sorry
-theorem add_right_inv : a + -a = 0                := by sorry
+-- NOTE: Using `@add_assoc` etc, produces `.proj` expressions.
+
+-- https://leanprover.zulipchat.com/#narrow/stream/270676-lean4/topic/elabTerm.20with.20TC
+
+theorem t [Add α] (a b : α) : a + b = b + a :=
+  sorry
+
+set_option trace.egg true
+
+-- TODO: This example shows that we're not treating level params correctly, as they're hindering the
+--       rewriting. Can we replace all universe params by mvars such that the same param maps to the
+--       same mvar in all rewrites?
+example {a b : Nat} : a + b = b + a := by
+  egg [t]
+
+theorem inv_add_cancel_left'' : add (neg a) (add a b) = b := by
+  rw [←add_assoc]
+  rw [add_left_inv]
+  rw [zero_add]
+
+open Lean Meta Elab Term in
+#eval do
+  let e ← elabTerm (← `(t)) none
+  let ty ← inferType e
+  IO.println ty
+
+-- BUG: "type expected g"
+theorem inv_add_cancel_left' : -a + (a + b) = add (neg a) (add a b) := by
+  egg [@add_assoc, @zero_add, @add_zero, @add_left_inv, @add_right_inv]
 
 theorem inv_add_cancel_left : -a + (a + b) = b := by
-  egg [add_assoc, zero_add, add_zero, add_left_inv, add_right_inv]
+  egg [@add_assoc, @zero_add, @add_zero, @add_left_inv, @add_right_inv]
 
 theorem add_inv_cancel_left : a + (-a + b) = b := by
   egg [add_assoc, zero_add, add_zero, add_left_inv, add_right_inv]
