Lean/Egg/Core/Basic.lean
@@ -11,14 +11,25 @@ private opaque explainCongrC
   (lhs rhs : Expression) (rwNames : Array String) (lhss rhss : Array Egg.Expression)
   (dirs : Array Directions) (optimizeExpl : Bool) : String
 
+-- TODO: Clean this up.
+
 -- Note: We wrap this in an `IndexT` so that we can trace the type indices later.
 def explainCongr (cgr : Congr) (rws : Rewrites) (dirs : Array Directions) (cfg : Config) :
-    IndexT MetaM String := do
-  let names := rws.map (·.src.description)
-  let lhs    ← cgr.lhs.toEgg! .goal cfg
-  let rhs    ← cgr.rhs.toEgg! .goal cfg
-  let lhss   ← rws.mapM (·.lhs.toEgg! .rw cfg)
-  let rhss   ← rws.mapM (·.rhs.toEgg! .rw cfg)
+    IndexT MetaM (String × Rewrites × Array Directions) := do
+  let lhs     ← cgr.lhs.toEgg .goal cfg
+  let rhs     ← cgr.rhs.toEgg .goal cfg
+  let rwLhss  ← rws.mapM fun rw => rw.lhs.toEgg rw.src cfg
+  let rwRhss  ← rws.mapM fun rw => rw.rhs.toEgg rw.src cfg
+  let (tcProjs, tcDirs) := Array.unzip <| ← (← IndexT.getTcProjReductions).filterMapM fun rw => do
+    let some dirs ← rw.validDirs cfg.eraseULvls | return none
+    return some (rw, dirs)
+  let names  := (rws ++ tcProjs).map (·.src.description)
+  let dirs   := dirs ++ tcDirs
+  let tcLhss  ← tcProjs.mapM fun rw => rw.lhs.toEgg rw.src { cfg with genTcProjRws := false }
+  let tcRhss  ← tcProjs.mapM fun rw => rw.rhs.toEgg rw.src { cfg with genTcProjRws := false }
+  let lhss   := rwLhss ++ tcLhss
+  let rhss   := rwRhss ++ tcRhss
+  let allRws := rws ++ tcProjs
   if cfg.exitPoint == .beforeEqSat
-  then return ""
-  else return explainCongrC lhs rhs names lhss rhss dirs cfg.optimizeExpl
+  then return ("", allRws, dirs)
+  else return (explainCongrC lhs rhs names lhss rhss dirs cfg.optimizeExpl, allRws, dirs)
