Lean/Egg/Core/Encode/Basic.lean
@@ -3,27 +3,27 @@ import Egg.Core.Encode.EncodeM
 
 namespace Lean
 
--- Note: The encoding of expression mvars and universe level mvars in rewrites relies on the fact
---       that their indices are also unique between eachother.
-
-def Level.toEgg! : Level → Egg.Expression.Kind → Egg.Expression
-  | .zero,       _     => "0"
-  | .succ l,     k     => s!"(succ {l.toEgg! k})"
-  | .max l₁ l₂,  k     => s!"(max {l₁.toEgg! k} {l₂.toEgg! k})"
-  | .imax l₁ l₂, k     => s!"(imax {l₁.toEgg! k} {l₂.toEgg! k})"
-  | .mvar id,    .goal => s!"(uvar {id.uniqueIdx!})"
-  | .mvar id,    .rw   => s!"?{id.uniqueIdx!}"
-  | .param name, _     => s!"(param {name})"
-
-open Egg (EncodeM IndexT)
+open Egg (Expression Source EncodeM IndexT)
 open Egg.EncodeM
 open Egg.IndexT
 
-partial def Expr.toEgg! (e : Expr) (kind : Egg.Expression.Kind) (cfg : Egg.Config) :
-    IndexT MetaM Egg.Expression :=
-  Prod.fst <$> (go e).run { exprKind := kind, config := cfg }
+-- Note: The encoding of expression mvars and universe level mvars in rewrites relies on the fact
+--       that their indices are also unique between eachother.
+
+-- BUG?: Should params be encoded as (coordinated) mvars within rewrites?
+def Level.toEgg : Level → Source → MetaM Egg.Expression
+  | .zero,       _     => return "0"
+  | .succ l,     k     => return s!"(succ {← l.toEgg k})"
+  | .max l₁ l₂,  k     => return s!"(max {← l₁.toEgg k} {← l₂.toEgg k})"
+  | .imax l₁ l₂, k     => return s!"(imax {← l₁.toEgg k} {← l₂.toEgg k})"
+  | .mvar id,    .goal => return s!"(uvar {id.uniqueIdx!})"
+  | .mvar id,    _     => return s!"?{id.uniqueIdx!}"
+  | .param name, _     => return s!"(param {name})"
+
+partial def Expr.toEgg (e : Expr) (src : Source) (cfg : Egg.Config) : IndexT MetaM Expression :=
+  Prod.fst <$> (go e).run { exprSrc := src, config := cfg }
 where
-  go (e : Expr) : EncodeM Egg.Expression := do
+  go (e : Expr) : EncodeM Expression := do
     if ← needsProofErasure e then return "proof" else
       let c ← encode e
       -- TODO: What happens here when we have a leading `mdata`?
@@ -31,7 +31,7 @@ where
         let some tag ← getTypeTag? e | unreachable!
         return s!"(τ {tag} {c})"
 
-  getTypeTag? (e : Expr) : EncodeM (Option Egg.Expression) := do
+  getTypeTag? (e : Expr) : EncodeM (Option Expression) := do
     let ty ← Meta.inferType e
     match (← config).typeTags with
     | .indices => return s!"{← typeIdx ty}"
@@ -39,32 +39,50 @@ where
     | .none    => return none
 
   -- TODO: Reconsider how to handle the binder type of a `forallE` in the typed and untyped settings.
-  encode : Expr → EncodeM Egg.Expression
+  encode : Expr → EncodeM Expression
     | bvar idx         => return s!"(bvar {idx})"
     | fvar id          => encodeFVar id
     | mvar id          => encodeMVar id
-    | sort lvl         => return s!"(sort {lvl.toEgg! (← exprKind)})"
-    | const name lvls  => return s!"(const {name}{← encodeULvls lvls})"
-    | app fn arg       => return s!"(app {← go fn} {← go arg})"
-    | lam _ ty b _     => withInstantiatedBVar ty b (return s!"(λ {← go ·})")
-    | forallE _ ty b _ => withInstantiatedBVar ty b (return s!"(∀ {← go ty} {← go ·})")
+    | sort lvl         => return s!"(sort {← lvl.toEgg (← exprSrc)})"
+    | const name lvls  => encodeConst name lvls
+    | app fn arg       => encodeApp fn arg
+    | lam _ ty b _     => withEmptyAppArgs do withInstantiatedBVar ty b (return s!"(λ {← go ·})")
+    | forallE _ ty b _ => withEmptyAppArgs do withInstantiatedBVar ty b (return s!"(∀ {← go ty} {← go ·})")
     | lit (.strVal l)  => return s!"(lit \"{l}\")"
     | lit (.natVal l)  => return s!"(lit {l})"
     | mdata _ e        => go e
     | e@(letE ..)      => do go (← Meta.zetaReduce e)
-    | proj ..          => panic! "egg: tried to encode projection"
+    | proj ty ctor b   => encodeProj ty ctor b
 
-  encodeMVar (id : MVarId) : EncodeM Egg.Expression := do
-    match ← exprKind with
-    | .goal => return s!"(mvar {id.uniqueIdx!})"
-    | .rw   => return s!"?{id.uniqueIdx!}"
-
-  encodeFVar (id : FVarId) : EncodeM Egg.Expression := do
+  encodeFVar (id : FVarId) : EncodeM Expression := do
     if let some bvarIdx ← bvarIdx? id
     then return s!"(bvar {bvarIdx})"
     else return s!"(fvar {id.uniqueIdx!})"
 
+  encodeMVar (id : MVarId) : EncodeM Expression := do
+    match ← exprSrc with
+    | .goal => return s!"(mvar {id.uniqueIdx!})"
+    | _     => return s!"?{id.uniqueIdx!}"
+
+  encodeConst (name : Name) (lvls : List Level) : EncodeM Expression := do
+    saveTcProjIfApplicable name lvls
+    return s!"(const {name}{← encodeULvls lvls})"
+
+  encodeApp (fn arg : Expr) : EncodeM Expression := do
+    let eFn ← withAppArg arg do go fn
+    let eArg ← withEmptyAppArgs do go arg
+    return s!"(app {eFn} {eArg})"
+
+  encodeProj (ty : Name) (ctor : Nat) (b : Expr) : EncodeM Expression := do
+    let env ← getEnv
+    let some field := (getStructureFields env ty)[ctor]? | throwError "egg: failed to encode proj"
+    let some prj   := getProjFnForField? env ty field    | throwError "egg: failed to encode proj"
+    let some info  := env.find? prj                      | throwError "egg: failed to encode proj"
+    let lParams    := info.levelParams.map (Level.param ·)
+    let expr       := Expr.app (.const prj lParams) b
+    go expr
+
   encodeULvls (lvls : List Level) : EncodeM String := do
     if (← config).eraseULvls
     then return ""
-    else return lvls.foldl (init := "") (s!"{·} {·.toEgg! (← exprKind)}")
+    else lvls.foldlM (init := "") fun res lvl => return s!"{res} {← lvl.toEgg (← exprSrc)}"
