Lean/Egg/Core/Encode/Expression.lean
@@ -1,5 +1,0 @@
-abbrev Egg.Expression := String
-
-inductive Egg.Expression.Kind where
-  | goal
-  | rw
