Lean/Egg/Core/Expression.lean
@@ -1,0 +1,1 @@
+abbrev Egg.Expression := String
