Lean/Egg/Core/Source.lean
@@ -1,0 +1,24 @@
+import Egg.Lean
+import Lean
+open Lean
+
+namespace Egg
+
+inductive Source where
+  | goal
+  | explicit (idx : Nat) (eqn? : Option Nat)
+  | star (id : FVarId)
+  | tcProj (src : Source) (idx : Nat)
+  deriving Inhabited, BEq, Hashable
+
+namespace Source
+
+def description : Source → String
+  | .goal                    => s!"⊢"
+  | .explicit idx none       => s!"#{idx}"
+  | .explicit idx (some eqn) => s!"#{idx}/{eqn}"
+  | .star id                 => s!"*{id.uniqueIdx!}"
+  | .tcProj src idx          => s!"{src.description}[{idx}]"
+
+instance : ToString Source where
+  toString := description
