Lean/Egg/Core/TcProj.lean
@@ -1,0 +1,24 @@
+import Egg.Core.Rewrites
+import Lean
+open Lean Meta
+
+namespace Egg
+
+-- We expect the `args` to contain `numParams + 1` elements where the `numParams + 1`th argument is
+-- the type class instance argument for `const`.
+structure TcProj where
+  const : Name
+  lvls  : List Level
+  args  : Array Expr
+  deriving BEq, Hashable
+
+def TcProj.reductionRewrite? (proj : TcProj) (src : Source) : MetaM (Option Rewrite) := do
+  let some tcArg := proj.args.back? | return none
+  unless !tcArg.isMVar do return none
+  let app := mkAppN (.const proj.const proj.lvls) proj.args
+  let reduced := (← reduceAll app).eta
+  let eq ← mkEq app reduced
+  let proof ← mkEqRefl app
+  let some rw ← Rewrite.from? proof eq src false
+    | throwError "egg: internal error in 'TcProj.reductionRewrite?'"
+  return rw
