Test/Tests/Binders.lean
@@ -1,5 +1,7 @@
 import Egg
 
+-- TODO: These tests are broken because of typeclass rewrite generation.
+
 example : (fun x : Nat => 0) = (fun x => 0 + 0) := by
   egg [Nat.add_zero]
 
@@ -9,5 +11,6 @@ example : (fun x => x) = (fun x => x + 0) := by
 example (f : (Nat → Nat) → Bool) : f (fun x => x) = f (fun x => x + 0) := by
   egg [Nat.add_zero]
 
+set_option trace.egg true
 example (h : ∀ x y : Nat, x = y ↔ y = x) : (∀ x y : Nat, x = y) ↔ (∀ a b : Nat, b = a + 0) := by
   egg [h, Nat.add_zero]
